wip untyped semantics - unary operators ok

coq/UntypedSemantics.v
@@ -2,14 +2,28 @@
 Require Export Koika.Common Koika.Environments Koika.ULogs Koika.Syntax
   Koika.Syntax.
 
+
+Ltac destr_in H :=
+  match type of H with
+  | context[match ?a with _ => _ end] => destruct a eqn:?
+  end.
+
+Ltac destr :=
+  match goal with
+    |- context[match ?a with _ => _ end] => destruct a eqn:?; try congruence
+  end.
+
+Ltac inv H :=
+  inversion H; try subst; clear H.
+
 Section Interp.
   Context {pos_t var_t fn_name_t reg_t ext_fn_t: Type}.
   Context {reg_t_eq_dec: EqDec reg_t}.
   Context {var_t_eq_dec: EqDec var_t}.
 
   Inductive val :=
-  | Bits (n: nat) (v: bits n)
-  | Enum (sig: enum_sig) (v: bits (enum_bitsize sig))
+  | Bits (sz:nat) (v: list bool)
+  | Enum (sig: enum_sig) (v: list bool)
   | Struct (sig: struct_sig) (v: list val)
   | Array (sig: array_sig) (v: list val).
 
@@ -96,47 +110,74 @@ Section Interp.
            : list val :=
              match fields return struct_denote fields -> list val with
              | [] => fun _ => []
-             | (nm, tau) :: fields => fun '(x, xs) =>
-                 (val_of_value x) :: (val_of_struct_value xs)
+             | (nm, tau) :: fields =>
+               fun '(x, xs) =>
+                 val_of_value x :: (val_of_struct_value xs)
              end x) in
       match tau return type_denote tau -> val with
-      | bits_t _ => fun bs => Bits _ bs
-      | enum_t _ => fun bs => Enum _ bs
+      | bits_t sz => fun bs => Bits sz  (vect_to_list bs)
+      | enum_t sig => fun bs => Enum sig (vect_to_list bs)
       | struct_t sig => fun str => Struct sig (val_of_struct_value str)
       | array_t sig => fun v => Array sig (map val_of_value (vect_to_list v))
       end x.
 
-    Definition val_bits_app (v1 v2: val) : val :=
-      match v1, v2 with
-      | Bits _ b1, Bits _ b2 => Bits _ (Bits.app b1 b2)
-      | _, _ => Bits _ Ob
-      end.
-
-    Definition val_concat (l: list val) : val :=
-      fold_left (val_bits_app) l (Bits _ Ob).
-
-    Fixpoint ubits_of_value (v: val) : val :=
+    Fixpoint ubits_of_value (v: val) : list bool :=
       match v with
-      | Bits _ bs => Bits _ bs
-      | Enum _ bs => Bits _ bs
-      | Struct _ lv => val_concat (map ubits_of_value lv)
-      | Array _ lv => val_concat (map ubits_of_value lv)
+      | Bits _ bs => bs
+      | Enum _ bs => bs
+      | Struct _ lv => List.concat (rev (map ubits_of_value lv))
+      | Array _ lv => List.concat (rev (map ubits_of_value lv))
       end.
+
+    Lemma ubits_of_value_len:
+      forall {tau} (v: type_denote tau) bs,
+        ubits_of_value (val_of_value v) = bs ->
+        List.length bs = type_sz tau.
+    Proof.
+      fix IHt 1. destruct tau; simpl; intros; subst.
+      apply vect_to_list_length.
+      apply vect_to_list_length.
+      - revert sig v. destruct sig. simpl.
+        induction struct_fields; simpl; intros.
+        + subst. reflexivity.
+        + destruct a. destruct v. simpl.
+          rewrite List.concat_app. simpl.
+          rewrite app_length. simpl.
+          rewrite IHstruct_fields.
+          unfold struct_fields_sz. simpl. f_equal.
+          rewrite app_nil_r.
+          eapply IHt; eauto.
+      - revert sig v. destruct sig. simpl. intros.
+        induction array_len; simpl. auto.
+        destruct v. simpl.
+        rewrite concat_app. rewrite app_length. simpl.
+        unfold vect_to_list in IHarray_len. rewrite IHarray_len.
+        clear IHarray_len. f_equal. rewrite app_nil_r. eapply IHt. eauto.
+    Qed.
 
     Lemma ubits_of_value_ok:
       forall {tau} (v: type_denote tau) bs,
-        ubits_of_value (val_of_value v) = Bits _ bs ->
-        bits_of_value v = bs.
+        ubits_of_value (val_of_value v) = bs ->
+        vect_to_list (bits_of_value v) = bs.
     Proof.
-      induction tau; simpl; intros.
-      - inversion H.
-        apply Eqdep_dec.inj_pair2_eq_dec in H1. 2: apply eq_dec. auto.
-      - inversion H.
-        apply Eqdep_dec.inj_pair2_eq_dec in H1. 2: apply eq_dec. auto.
-      (*
-      - induction struct_fields.
-        + cbn in H. injection H.
-      *) Admitted.
+      fix IHt 1. destruct tau; simpl; intros; subst; auto.
+      - revert sig v. destruct sig. simpl.
+        induction struct_fields; simpl; intros.
+        + subst. reflexivity.
+        + destruct a. destruct v. simpl.
+          rewrite List.concat_app. simpl.
+          rewrite <- IHstruct_fields. rewrite app_nil_r.
+          simpl in *.
+          rewrite <- (IHt _ t0 _ eq_refl).
+          rewrite <- vect_to_list_app.
+          reflexivity.
+      - revert sig v. destruct sig. simpl. intros.
+        induction array_len; simpl. auto.
+        destruct v. simpl.
+        rewrite vect_to_list_app. rewrite IHarray_len. clear IHarray_len.
+        rewrite concat_app. f_equal. simpl.
+        rewrite app_nil_r. eapply IHt. eauto.
+    Qed.
 
     Fixpoint replace {sig: tsig var_t} k (v: val) (Gamma: tcontext sig)
       : tcontext sig
@@ -158,107 +199,998 @@ Section Interp.
       exact (Some (v0, v1)).
     Defined.
 
-    Definition val_split (n: nat) (v: val) : option (val * val) :=
-      match v with
-      | Bits sz bs =>
-        let/opt2 b0, b1 := bits_split n bs in
-        Some (Bits _ b0, Bits _ b1)
-      | _ => None
+    Fixpoint take_drop {A: Type} (n: nat) (l: list A) : option (list A * list A) :=
+      match n with
+        O => Some ([], l)
+      | S n =>
+        match l with
+          [] => None
+        | a::l =>
+          let/opt2 l1, l2 := take_drop n l in
+          Some (a::l1, l2)
+        end
       end.
 
-    Fixpoint bits_splitn {sz} (nb sz_elt: nat) (bs: bits sz)
-      : option (list (bits sz_elt))
+    Definition take_drop' {A: Type} n (l: list A) :=
+      match take_drop n l with
+        None => (l,[])
+      | Some (l1, l2) => (l1, l2)
+      end.
+
+    Fixpoint bits_splitn (nb sz_elt: nat) (bs: list bool)
+      : option (list (list bool))
     :=
       match nb with
         O => Some []
       | S nb =>
-        let/opt2 hd, rest := bits_split sz_elt bs in
+        let/opt2 hd, rest := take_drop sz_elt bs in
         let/opt tl := bits_splitn nb sz_elt rest in
         Some (hd :: tl)
       end.
 
-    Definition bits_of_bits (n1: nat) {n} (bs: bits n) : option (bits n1).
-      destruct (eq_dec n n1). subst.
-      exact (Some bs).
-      exact None.
-    Defined.
+    Lemma take_drop_succeeds:
+      forall {A:Type} (n: nat) (l: list A) (LT: n <= Datatypes.length l),
+      exists la lb,
+        take_drop n l = Some (la, lb).
+    Proof.
+      induction n; simpl; intros; eauto.
+      destruct l; simpl in LT. lia.
+      destruct (IHn l) as (la & lb & EQ). lia.
+      rewrite EQ. simpl.
+      eauto.
+    Qed.
 
-    Definition enum_of_bits (sig: enum_sig) {n} (bs: bits n)
-      : option (bits (enum_bitsize sig))
-    :=
-      bits_of_bits (enum_bitsize sig) bs.
+    Lemma take_drop_spec:
+      forall {A:Type} (n: nat) (l la lb: list A),
+        take_drop n l = Some (la, lb) ->
+        l = la ++ lb /\ List.length la = n /\ List.length lb = List.length l - n.
+    Proof.
+      induction n; simpl; intros; eauto.
+      inversion H; clear H; subst. repeat split; try reflexivity. lia.
+      destruct l. congruence.
+      destruct (take_drop n l) eqn:EQ; simpl in H; try congruence.
+      destruct p. inversion H; clear H; subst.
+      apply IHn in EQ. destruct EQ as (EQ1 & EQ2 & EQ3). subst. simpl.
+      repeat split; lia.
+    Qed.
 
-    Fixpoint value_of_bits {tau: type} (bs: val) {struct tau}: option val :=
-      let value_of_struct_bits :=
-        (fix value_of_struct_bits
+    Lemma take_drop'_cons:
+      forall {A} (l l1 l2: list A) a n,
+      take_drop' n l = (l1, l2) ->
+      take_drop' (S n) (a::l) = (a::l1, l2).
+    Proof.
+      unfold take_drop'. simpl. intros. destruct (take_drop n l) eqn:?.
+      - destruct p. inversion H; subst. simpl. auto.
+      - simpl. inversion H; subst. auto.
+    Qed.
+
+    Lemma take_drop'_spec:
+      forall {A:Type} (n: nat) (l la lb: list A),
+        take_drop' n l = (la, lb) ->
+        l = la ++ lb /\ List.length la <= n /\ List.length lb = List.length l - List.length la.
+    Proof.
+      induction n; simpl; intros; eauto.
+      inversion H; clear H; subst. repeat split; try reflexivity. simpl; lia.
+      destruct l; simpl in *. unfold take_drop' in H. simpl in *. inversion H; clear H.
+      simpl. repeat split; lia.
+      destruct (take_drop' n l) as (l1 & l2) eqn:?.
+      erewrite take_drop'_cons in H; eauto. inversion H; subst. simpl.
+      apply IHn in Heqp. destruct Heqp as (EQ1 & EQ2 & EQ3). subst.
+      repeat split; auto. lia.
+    Qed.
+
+
+    Lemma app_eq_inv:
+      forall {A:Type} (a b c d: list A),
+        a ++ b = c ++ d ->
+        List.length a = List.length c ->
+        a = c /\ b = d.
+    Proof.
+      induction a; simpl; intros; eauto.
+      - destruct c; simpl in H0; try congruence.
+        simpl in *. auto.
+      - destruct c; simpl in H0; try congruence.
+        simpl in *. inversion H; clear H; subst.
+        apply IHa in H3. destruct H3; subst; auto. lia.
+    Qed.
+
+    Inductive wt_val: type -> val -> Prop :=
+    | wt_bits: forall n bs,
+        List.length bs = n ->
+        wt_val (bits_t n) (Bits n bs)
+    | wt_enum: forall sig bs,
+        List.length bs = enum_bitsize sig ->
+        wt_val (enum_t sig) (Enum sig bs)
+    | wt_struct: forall sig lv,
+        Forall2 (fun nt v => wt_val nt v) (map snd (struct_fields sig)) lv ->
+        wt_val (struct_t sig) (Struct sig lv)
+    | wt_array: forall sig lv,
+        Forall (fun v => wt_val (array_type sig) v) lv ->
+        List.length lv = array_len sig ->
+        wt_val (array_t sig) (Array sig lv).
+
+    Fixpoint size_type (t: type) :=
+      match t with
+      | bits_t n => 1
+      | enum_t sig => 1
+      | struct_t sig =>
+        1 + list_sum (List.map (fun '(_, t) => size_type t) (struct_fields sig))
+      | array_t sig =>
+        1 + size_type (array_type sig)
+      end.
+
+    Lemma wt_val_ind':
+      forall (P : type -> val -> Prop)
+       (Hbits: forall (n : nat) (bs : list bool), Datatypes.length bs = n -> P (bits_t n) (Bits n bs))
+       (Henum: forall (sig : enum_sig) (bs : list bool),
+        Datatypes.length bs = enum_bitsize sig -> P (enum_t sig) (Enum sig bs))
+       (Hstruct: forall (sig : struct_sig) (lv : list val),
+        Forall2 (fun (nt : type) (v : val) => wt_val nt v) (map snd (struct_fields sig)) lv ->
+        Forall2 (fun (nt : type) (v : val) => wt_val nt v -> P nt v) (map snd (struct_fields sig)) lv ->
+        P (struct_t sig) (Struct sig lv))
+       (Harray: forall (sig : array_sig) (lv : list val),
+        Forall (fun v : val => wt_val (array_type sig) v) lv ->
+        Forall (fun v : val => wt_val (array_type sig) v -> P (array_type sig) v) lv ->
+        Datatypes.length lv = array_len sig -> P (array_t sig) (Array sig lv)),
+      forall (t : type) (v : val), wt_val t v -> P t v.
+    Proof.
+      intros P Hbits Henum Hstruct Harray t v.
+      remember (size_type t).
+      revert t v Heqn.
+      pattern n.
+      eapply Nat.strong_right_induction with (z:=0).
+      {
+        red. red. intros. subst. tauto.
+      } 2: lia.
+      intros n0 _ Plt t t0 a Heqn.
+      assert (Plt':
+                forall t v,
+                  size_type t < n0 -> wt_val t v -> P t v
+             ).
+      {
+        intros. eapply Plt. 3: reflexivity. lia. auto. auto.
+      } clear Plt.
+      rename Plt' into Plt.
+      subst.
+      inversion Heqn; subst; eauto.
+      - eapply Hstruct. eauto.
+        revert H.
+        simpl in Plt.
+        assert (Forall (fun '(n,t) => forall v, wt_val t v -> P t v) (struct_fields sig)).
+        {
+          revert Plt; clear. destruct sig. simpl.
+          induction struct_fields; simpl; intros. constructor.
+          constructor; eauto. destruct a; simpl; intros.
+          eapply Plt. lia. auto.
+          apply IHstruct_fields.
+          intros; eapply Plt; eauto. lia.
+        }
+        clear Heqn. revert H lv. clear Plt.
+        destruct sig. simpl. clear.
+        induction 1; simpl; intros; eauto. inv H. constructor.
+        inv H1.
+        constructor; auto. destruct x; simpl in *; eauto.
+      - eapply Harray; eauto.
+        rewrite Forall_forall. intros x IN WT.
+        eapply Plt; eauto.
+    Qed.
+
+    Fixpoint size_val (v: val) :=
+      match v with
+      | Bits _ _ => 1
+      | Enum _ _ => 1
+      | Struct sig lv => 1 + list_sum (map size_val lv)
+      | Array sig lv => 1 + list_sum (map size_val lv)
+      end.
+
+
+
+    Lemma take_drop_succeeds_eq:
+      forall {A:Type} (n: nat) (l: list A) (LT: n = Datatypes.length l),
+        take_drop n l = Some (l, []).
+    Proof.
+      induction n; simpl; intros; eauto.
+      destruct l; simpl in LT. reflexivity. lia.
+      destruct l; simpl in LT; try lia.
+      rewrite IHn; simpl; auto.
+    Qed.
+
+    Lemma take_drop_head:
+      forall {A} n (l1 l2: list A),
+        n = List.length l1 ->
+        take_drop n (l1 ++ l2) = Some (l1, l2).
+    Proof.
+      intros. subst. revert l2.
+      induction l1; simpl; intros; subst; eauto.
+      rewrite IHl1. simpl. reflexivity.
+    Qed.
+
+    Lemma length_concat_same:
+      forall {A} (l: list (list A)) sz,
+        Forall (fun x => List.length x = sz) l ->
+        Datatypes.length (List.concat l) = List.length l * sz.
+    Proof.
+      induction 1; simpl; intros; eauto.
+      rewrite app_length; rewrite IHForall. lia.
+    Qed.
+
+
+    Lemma ubits_of_value_len':
+      forall tau v,
+        wt_val tau v ->
+        List.length (ubits_of_value v) = type_sz tau.
+    Proof.
+      intros tau v WT.
+      pattern tau, v.
+      eapply wt_val_ind'; simpl; intros; eauto.
+      - revert sig lv H0 H. destruct sig. simpl.
+        induction struct_fields; simpl; intros.
+        + inv H0. reflexivity.
+        + inv H0. inv H. simpl.
+          rewrite concat_app, app_length. simpl.
+          rewrite app_nil_r. rewrite H3; auto.
+          erewrite IHstruct_fields. reflexivity. eauto. auto.
+      - rewrite Bits.rmul_correct. erewrite length_concat_same.
+        rewrite rev_length. rewrite map_length. rewrite H1. reflexivity.
+        rewrite Forall_forall in *.
+        intros x IN. subst.
+        apply In_rev in IN.
+        rewrite in_map_iff in IN. destruct IN as (x0 & EQ & IN); subst.
+        eapply H0. auto. eauto.
+    Qed.
+
+    Lemma bits_splitn_concat:
+      forall sz l n,
+        Forall (fun l => List.length l = sz) l ->
+        List.length l = n ->
+        bits_splitn n sz (List.concat l) = Some l.
+    Proof.
+      intros. subst.
+      induction H; simpl; intros; auto.
+      rewrite take_drop_head; auto. simpl.
+      rewrite IHForall. simpl. reflexivity.
+    Qed.
+
+
+    Fixpoint uvalue_of_bits {tau: type} (bs: list bool) {struct tau}: option val :=
+      let uvalue_of_struct_bits :=
+        (fix uvalue_of_struct_bits
              {fields: list (string * type)}
-             (bs: val)
+             (bs: list bool)
          : option (list val) :=
            match fields with
            | [] => Some []
            | (nm, tau) :: fields =>
-             let/opt2 b0, b1 := val_split (type_sz tau) bs in
-             let/opt hd := value_of_bits (tau:=tau) b0 in
-             let/opt tl := value_of_struct_bits (fields:=fields) b1 in
-             Some (hd :: tl)
+             let/opt2 b0, b1 := take_drop (List.length bs - type_sz tau) bs in
+             let/opt tl := uvalue_of_struct_bits (fields:=fields) b0 in
+             let/opt hd := uvalue_of_bits (tau:=tau) b1 in
+             Some ( hd :: tl)
            end) in
-      let value_of_list_bits tau :=
-        fix value_of_list_bits {sz} (l : list (bits sz))
+      let uvalue_of_list_bits tau :=
+        fix uvalue_of_list_bits (l : list (list bool))
           : option (list val)
         :=
           match l with
           | [] => Some []
           | hd::tl =>
-            let/opt hd := value_of_bits (tau:=tau) (Bits _ hd) in
-            let/opt tl := value_of_list_bits tl in
+            let/opt hd := uvalue_of_bits (tau:=tau) hd in
+            let/opt tl := uvalue_of_list_bits tl in
             Some (hd::tl)
           end in
-      match bs with
-        Bits _ bs' =>
-        match tau with
-        | bits_t _ => Some bs
-        | enum_t sig => option_map (fun bs => Bits _ bs) (enum_of_bits sig bs')
-        | struct_t sig => option_map (fun lv => Struct sig lv)
-            (value_of_struct_bits (fields:=struct_fields sig) bs)
-        | array_t sig =>
-          let/opt lbs := bits_splitn (array_len sig)
-            (type_sz (array_type sig)) bs' in
-          let/opt lv := value_of_list_bits (array_type sig) lbs in
-          Some (Array sig lv)
-        end
+      match tau with
+      | bits_t _ => Some (Bits (Datatypes.length bs) bs)
+      | enum_t sig =>
+        let/opt2 b0, b1 := take_drop (enum_bitsize sig) bs in
+        (* TODO check b1 is empty ? *)
+        Some (Enum sig b0)
+      | struct_t sig =>
+        let/opt lv := uvalue_of_struct_bits (fields:=struct_fields sig) bs in
+        Some (Struct sig lv)
+      | array_t sig =>
+        let/opt lbs := bits_splitn (array_len sig)
+                                   (type_sz (array_type sig)) bs in
+        let/opt lv := uvalue_of_list_bits (array_type sig) (rev lbs) in
+        Some (Array sig lv)
+      end
+    .
+
+
+    Lemma uvalue_of_bits_val:
+      forall tau v,
+        wt_val tau v ->
+        uvalue_of_bits (tau:=tau) (ubits_of_value v) =
+        Some v.
+    Proof.
+      intros tau v WT.
+      pattern tau, v.
+      eapply wt_val_ind'; simpl; intros; eauto.
+      - congruence.
+      - rewrite take_drop_succeeds_eq; simpl; auto.
+      - revert sig lv H H0. destruct sig. simpl.
+        induction struct_fields; simpl; intros.
+        + inv H. reflexivity.
+        + inv H. inv H0. destruct a. simpl in *.
+          rewrite concat_app, app_length. simpl. 
+          rewrite app_nil_r.
+          erewrite ubits_of_value_len'. 2: eauto.
+          rewrite take_drop_head. 2: lia. simpl.
+          generalize (IHstruct_fields l' H5 H7). intro A.
+          match type of A with
+            context[ let/opt _ := ?a in _ ] => destruct a eqn:?
+          end; simpl in *; try congruence.
+          rewrite H4. simpl. inv A; auto. auto.
+      -
+        assert (Forall (fun v => wt_val (array_type sig) v /\ uvalue_of_bits (tau:= array_type sig) (ubits_of_value v) = Some v) lv).
+        {
+          rewrite Forall_forall in *; simpl; intros.
+          split; eauto.
+        }
+        clear H H0.
+
+        rewrite bits_splitn_concat.
+        simpl.
+        rewrite rev_involutive.
+        cut ((fix uvalue_of_list_bits (l : list (list bool)) : option (list val) :=
+         match l with
+         | [] => Some []
+         | hd :: tl =>
+             let/opt hd0 := uvalue_of_bits (tau:=array_type sig) hd
+             in (let/opt tl0 := uvalue_of_list_bits tl in Some (hd0 :: tl0))
+         end) ((map ubits_of_value lv)) = Some lv).
+        intro A; rewrite A. simpl. reflexivity.
+        revert H1 H2. generalize lv (array_len sig). clear.
+        intros l n EQ. subst. revert l.
+        induction l; simpl; intros; eauto.
+        inv H2. destruct H1. rewrite H0. simpl.
+        rewrite IHl. simpl. auto. auto.
+        rewrite Forall_forall in *. intros x IN.
+        apply In_rev in IN.
+        rewrite in_map_iff in IN. destruct IN as (xx & EQ & IN). subst.
+        erewrite ubits_of_value_len'. eauto.
+        apply H2. auto. rewrite rev_length, map_length; auto.
+    Qed.
+
+    (* Lemma struct_eq: *)
+    (*   forall fields x, *)
+    (*     rev ((fix *)
+    (*            val_of_struct_value (fields : list (string * type)) (x : struct_denote fields) {struct *)
+    (*                                                                                              fields} : list val := *)
+    (*            match fields as fields0 return (struct_denote fields0 -> list val) with *)
+    (*            | [] => fun _ : unit => [] *)
+    (*            | p :: fields0 => *)
+    (*              let (_, tau) as p0 return (snd p0 * struct_denote fields0 -> list val) := p in *)
+    (*              fun '(x0, xs) => val_of_value x0 :: val_of_struct_value fields0 xs *)
+    (*            end x) fields x) =  *)
+    (*     (fix *)
+    (*        val_of_struct_value (fields : list (string * type)) (x : struct_denote fields) {struct *)
+    (*                                                                                          fields} : list val := *)
+    (*        match fields as fields0 return (struct_denote fields0 -> list val) with *)
+    (*        | [] => fun _ : unit => [] *)
+    (*        | p :: fields0 => *)
+    (*          let (_, tau) as p0 return (snd p0 * struct_denote fields0 -> list val) := p in *)
+    (*          fun '(x0, xs) => [val_of_value x0] ++ val_of_struct_value fields0 xs *)
+    (*        end x) fields x. *)
+    (* Proof. *)
+    (*   induction fields. reflexivity. intros. *)
+    (*   destruct a. destruct x. *)
+    (*   rewrite rev_app_distr. simpl. f_equal. eauto. *)
+    (* Qed. *)
+
+    Lemma wt_val_of_value:
+      forall (tau: type) (v: tau),
+        wt_val tau (val_of_value v).
+    Proof.
+      fix IHt 1. destruct tau; simpl; intros.
+      - constructor. rewrite vect_to_list_length. auto.
+      - constructor. rewrite vect_to_list_length. auto.
+      - eapply wt_struct.
+        revert v. generalize (struct_fields sig).
+        induction l; simpl; intros; eauto.
+        destruct a. destruct v. simpl. constructor. apply IHt.
+        eauto.
+      - eapply wt_array.
+        rewrite Forall_forall. intros x IN.
+        rewrite in_map_iff in IN.
+        destruct IN as (xx & EQ & IN). subst.
+        apply IHt.
+        rewrite map_length.
+        rewrite vect_to_list_length. auto.
+    Qed.
+
+
+    Lemma uvalue_of_bits_val':
+      forall tau v,
+        uvalue_of_bits (tau:=tau) (ubits_of_value (val_of_value (tau:=tau) v)) =
+        Some (val_of_value (tau:=tau) v).
+    Proof.
+      intros.
+      apply uvalue_of_bits_val.
+      apply wt_val_of_value.
+    Qed.
+
+    Locate CircuitPrimSpecs.sigma1.
+
+    Compute vect_of_list [true; true; false].
+
+    Import PrimUntyped.
+    Definition usigma1' (fn: PrimUntyped.ubits1) (bs: list bool) : option (list bool) :=
+      match fn with
+      | UNot => Some (List.map negb bs)
+      | USExt w =>
+        let msb := List.last bs false in
+        Some (bs ++ List.repeat msb (w - List.length bs))
+      | UZExtL w =>
+        Some (bs ++ List.repeat false (w - List.length bs))
+      | UZExtR w =>
+        Some (List.repeat false (w - List.length bs) ++ bs)
+      | URepeat times =>
+        Some (List.concat (List.repeat bs times))
+      | USlice ofs w =>
+        let '(_, bs) := take_drop' ofs bs in
+        let '(bs, _) := take_drop' w bs in
+        Some (bs ++ List.repeat false (w - List.length bs))
+      end.
+
+    Definition usigma1 fn v : option val :=
+      match v with
+        Bits _ bs =>
+        let/opt res := usigma1' fn bs in
+        Some (Bits (List.length res) res)
       | _ => None
       end.
 
+    Fixpoint get_field_struct (s: list (string * type)) (lv: list val) f : option val :=
+      match s, lv with
+      | (n, _)::s, a::lv =>
+        if eq_dec n f
+        then Some a
+        else get_field_struct s lv f
+      | _, _ => None
+      end.
 
-      Locate CircuitPrimSpecs.sigma1.
-  Definition sigma1 (fn: PrimUntyped.ufn1) : val -> option val :=
+    (* Fixpoint find_field (s: list (string * type)) f : option (nat * nat) := *)
+    (*   match s with *)
+    (*   | (n, t)::s => *)
+    (*     if eq_dec f n *)
+    (*     then Some (0, type_sz t) *)
+    (*     else *)
+    (*       let/opt2 ofs, sz := find_field s f in *)
+    (*       Some (ofs + type_sz t, sz) *)
+    (*   | _ => None *)
+    (*   end. *)
+
+
+    Fixpoint find_field_offset_right (s: list (string * type)) f : option (nat * nat) :=
+      match s with
+      | (n, t)::s =>
+        if eq_dec f n
+        then
+          Some (struct_fields_sz s, type_sz t)
+        else
+          find_field_offset_right s f
+      | [] => None
+      end.
+
+
+
+    Definition get_field (s: val) f : option val :=
+      match s with
+        Struct sig lv =>
+        get_field_struct (struct_fields sig) lv f
+      | _ => None
+      end.
+
+    Definition sigma1 (fn: PrimUntyped.ufn1) : val -> option val :=
+      match fn with
+      | PrimUntyped.UDisplay fn =>
+        match fn with
+        | PrimUntyped.UDisplayUtf8 => fun _ => Some (Bits 0 [])
+        | PrimUntyped.UDisplayValue _ => fun _ => Some (Bits 0 [])
+        end
+      | PrimUntyped.UConv fn =>
+        match fn with
+        | PrimUntyped.UPack => fun v =>
+                                 let bs := ubits_of_value v in
+                                 Some (Bits (List.length bs) bs)
+        | PrimUntyped.UUnpack tau =>
+          fun bs =>
+            match bs with
+            | Bits _ bs => let/opt v := uvalue_of_bits (tau:=tau) bs in Some v
+            | _ => None
+            end
+        | PrimUntyped.UIgnore => fun _ => Some (Bits 0 [])
+        end
+      | PrimUntyped.UBits1 fn => usigma1 fn
+      | PrimUntyped.UStruct1 (PrimUntyped.UGetField f) =>
+        fun v => get_field v f
+      | PrimUntyped.UStruct1 (UGetFieldBits sig f) =>
+        fun v =>
+          let/opt2 ofs, sz := find_field_offset_right (struct_fields sig) f in
+          usigma1 (USlice ofs sz) v
+      | PrimUntyped.UArray1 (PrimUntyped.UGetElement idx) =>
+        fun v =>
+          match v with
+          | Array sig l =>
+            List.nth_error l idx
+          | _ => None
+          end
+      | PrimUntyped.UArray1 (PrimUntyped.UGetElementBits sig idx) =>
+        fun v =>
+          usigma1 (USlice (element_sz sig * (array_len sig - S idx)) (element_sz sig)) v
+      end.
+
+
+Lemma uvalue_of_bits_val_of_value:
+  forall (tau: type) (v: vect bool (type_sz tau)),
+    uvalue_of_bits (tau:=tau) (vect_to_list v) = Some (val_of_value (value_of_bits v)).
+Proof.
+  intros; rewrite <- uvalue_of_bits_val'. f_equal.
+  erewrite <- ubits_of_value_ok. 2: eauto.
+  rewrite bits_of_value_of_bits. auto.
+Qed.
+
+Lemma repeat_bits_const:
+  forall x n,
+    repeat x n = vect_to_list (Bits.const n x).
+Proof.
+  induction n; simpl; auto.
+  rewrite IHn. reflexivity.
+Qed.
+
+Lemma last_nth:
+  forall {A} d (l: list A),
+    last l d = nth (List.length l - 1) l d.
+Proof.
+  induction l; simpl; intros; eauto.
+  destr. simpl. auto.
+  rewrite IHl. simpl. rewrite Nat.sub_0_r. reflexivity.
+Qed.
+
+Lemma bits_nth_list:
+  forall s (v: vect bool s) idx,
+    Bits.nth v idx = nth (index_to_nat idx) (vect_to_list v) false.
+Proof.
+  induction s; intros. simpl in idx; easy.
+  unfold Bits.nth. destr. simpl. auto. fold @vect_nth.
+  rewrite IHs. destruct v.  simpl. reflexivity.
+Qed.
+
+Lemma msb_spec:
+  forall s (v: bits s),
+    Bits.msb v = last (vect_to_list v) false.
+Proof.
+  unfold Bits.msb. intros.
+  destr. destruct v. reflexivity.
+  rewrite vect_last_nth.
+  rewrite last_nth. rewrite vect_to_list_length.
+  simpl Nat.sub.
+  rewrite Nat.sub_0_r.
+  rewrite bits_nth_list. f_equal.
+  apply index_to_nat_of_nat.
+  apply index_of_nat_largest.
+Qed.
+
+
+          Lemma vect_extend_end_firstn:
+            forall x s' (v: bits (Nat.min x s')) d,
+              vect_to_list (vect_extend_end_firstn v d) =
+              vect_to_list (vect_extend_end v x d).
+          Proof.
+            unfold vect_extend_end_firstn.
+            intros. rewrite vect_to_list_eq_rect. auto.
+          Qed.
+
+          Lemma vect_to_list_cons:
+            forall e s (v: bits s),
+              vect_to_list (v~e) = e:: vect_to_list v.
+          Proof.
+            reflexivity.
+          Qed.
+
+          Lemma vect_firstn_to_list:
+            forall s (v: bits s) n,
+              vect_to_list (vect_firstn n v) = fst (take_drop' n (vect_to_list v)).
+          Proof.
+            induction s; simpl; intros. simpl in *. destruct v. destr; reflexivity.
+            destr. reflexivity.
+            erewrite <- vect_to_list_eq_rect.
+            Unshelve.
+            3: replace (Nat.min (S n0) (S s)) with (S (Nat.min n0 s)); reflexivity.
+            simpl.
+            rewrite vect_to_list_cons.
+            rewrite IHs.
+            destruct v. simpl.
+            cbn. unfold take_drop'. simpl. unfold vect_to_list.
+            destr. destruct p. simpl. reflexivity.
+            simpl. reflexivity.
+          Qed.
+
+          Lemma vect_skipn_to_list:
+            forall s (v: bits s) n,
+              vect_to_list (vect_skipn n v) = snd (take_drop' n (vect_to_list v)).
+          Proof.
+            induction s; simpl; intros. simpl in *. destruct v. destr; reflexivity.
+            destr. reflexivity.
+            rewrite IHs.
+            unfold take_drop'.
+            destruct v. simpl.
+            cbn. unfold vect_to_list.
+            destr. destruct p. simpl. reflexivity.
+            simpl. reflexivity.
+          Qed.
+
+          Lemma take_drop'_spec2:
+            forall {A:Type} (n: nat) (l la lb: list A),
+              take_drop' n l = (la, lb) ->
+              l = la ++ lb /\
+              List.length la = Nat.min n (List.length l).
+          Proof.
+            induction n; simpl; intros; eauto.
+            inversion H; clear H; subst. repeat split; try reflexivity.
+            destruct l; simpl in *. unfold take_drop' in H. simpl in *. inversion H; clear H.
+            simpl. repeat split; lia.
+            destruct (take_drop' n l) as (l1 & l2) eqn:?.
+            erewrite take_drop'_cons in H; eauto. inv H. simpl.
+            apply IHn in Heqp. destruct Heqp as (EQ1 & EQ2). subst.
+            repeat split; auto.
+          Qed.
+
+
+Lemma usigma1_correct:
+      forall ufn fn,
+        PrimTypeInference.tc1 ufn (arg1Sig (PrimSignatures.Sigma1 fn)) = Success fn ->
+        forall (arg: arg1Sig (PrimSignatures.Sigma1 fn)) ret,
+          PrimSpecs.sigma1 fn arg = ret ->
+          sigma1 ufn (val_of_value arg) = Some (val_of_value ret).
+    Proof.
+      destruct ufn; simpl; intros.
+      - destruct fn.
+        + destr_in H; try congruence. inv H. simpl in *. inv Heqr0. subst. reflexivity.
+        + subst. inv H.
+          revert arg. rewrite <- H1. simpl. 
+          intro arg. reflexivity.
+      - destruct fn.
+        + inv H. revert arg. rewrite <- H2. simpl.
+          intros. f_equal.
+          erewrite ubits_of_value_len; eauto. f_equal.
+          erewrite ubits_of_value_ok; eauto.
+        + inv H.
+          generalize (wt_val_of_value _ arg). simpl. inversion 1; subst.
+          rewrite uvalue_of_bits_val_of_value. simpl. auto.
+        + inv H. revert arg. rewrite <- H2. simpl.
+          intros. f_equal.
+      - subst. destr_in H. inv H. simpl in *. inv Heqr0.
+        revert arg. rewrite <- H0. simpl. destruct fn; simpl in *; intros.
+        + rewrite map_length. rewrite vect_to_list_length. f_equal.
+          f_equal. rewrite <- vect_to_list_map. f_equal.
+        + f_equal. f_equal.
+          * rewrite app_length.
+            rewrite repeat_length. rewrite vect_to_list_length. lia.
+          * unfold Bits.extend_end. simpl.
+            rewrite vect_to_list_eq_rect.
+            rewrite vect_to_list_app. f_equal.
+            rewrite vect_to_list_length.
+            rewrite repeat_bits_const. f_equal. f_equal.
+            rewrite msb_spec; auto.
+        + f_equal. f_equal.
+          * rewrite app_length.
+            rewrite repeat_length. rewrite vect_to_list_length. lia.
+          * unfold Bits.extend_end. simpl.
+            unfold eq_rect.
+            refine (match vect_extend_end_cast s width with
+                    | eq_refl => _
+                    end).
+            rewrite vect_to_list_app. f_equal.
+            rewrite vect_to_list_length.
+            rewrite repeat_bits_const. f_equal.
+        + f_equal. f_equal.
+          * rewrite app_length.
+            rewrite repeat_length. rewrite vect_to_list_length. lia.
+          * unfold Bits.extend_beginning. simpl.
+            unfold eq_rect.
+            refine (match vect_extend_beginning_cast s width with
+                    | eq_refl => _
+                    end).
+            rewrite vect_to_list_app. f_equal.
+            rewrite vect_to_list_length.
+            rewrite repeat_bits_const. f_equal.
+        + f_equal. f_equal.
+          * erewrite length_concat_same.
+            rewrite repeat_length. reflexivity.
+            rewrite Forall_forall; intros x IN.
+            apply repeat_spec in IN. subst. rewrite vect_to_list_length. lia.
+          * induction times; simpl; auto.
+            rewrite vect_to_list_app. f_equal. eauto.
+        + destruct (take_drop' offset (vect_to_list arg)) as (l1 & l2) eqn:Heq1.
+          destruct (take_drop' width l2) as (l3 & l4) eqn:Heq2. simpl.
+          f_equal. f_equal.
+          apply take_drop'_spec in Heq2.
+          apply take_drop'_spec in Heq1.
+          intuition subst.
+          rewrite app_length.
+          rewrite repeat_length. lia.
+          unfold Bits.slice.
+
+          rewrite vect_extend_end_firstn.
+          unfold Bits.extend_end.
+          rewrite vect_to_list_eq_rect.
+          rewrite vect_to_list_app.
+          rewrite vect_firstn_to_list.
+          rewrite vect_skipn_to_list.
+          rewrite Heq1. simpl. rewrite Heq2. simpl.
+          rewrite <- repeat_bits_const.
+          f_equal. f_equal. f_equal.
+
+          apply take_drop'_spec2 in Heq2. destruct Heq2 as (Heq21 & Heq22). rewrite Heq22.
+          apply take_drop'_spec2 in Heq1. destruct Heq1 as (Heq11 & Heq12).
+          cut (List.length l2 = s - List.length l1). intro A; rewrite A. rewrite Heq12.
+          rewrite vect_to_list_length. lia.
+          erewrite <- (vect_to_list_length (sz:=s)). rewrite Heq11.
+          rewrite app_length. lia.
+        + inv H.
+      - destr_in H.
+        + repeat destr_in H; inv H.
+          simpl in Heqr0. clear Heqr0. simpl in arg.
+          simpl PrimSpecs.sigma1.
+          simpl.
+          unfold PrimTypeInference.find_field in Heqr1. unfold opt_result in Heqr1.
+          destr_in Heqr1; inv Heqr1.
+          revert s0 Heqo arg. destruct s. simpl. clear.
+          induction struct_fields; intros; eauto. easy.
+          destruct a. destruct arg.
+          Opaque eq_dec.
+          simpl. simpl in Heqo.
+          destr_in Heqo. inv Heqo. simpl in *. rewrite Heqs2. auto.
+          destr.  subst. congruence.
+          destr_in Heqo; inv Heqo.
+          erewrite IHstruct_fields; eauto. reflexivity.
+        + destr_in H; inv H.
+          simpl PrimSpecs.sigma1.
+          simpl.
+
+          assert (
+              forall sig (i: index (List.length (struct_fields sig))),
+              PrimTypeInference.find_field sig f = Success i ->
+              find_field_offset_right (struct_fields sig) f = Some (field_offset_right sig i, field_sz sig i)
+            ).
+          {
+            clear. intros sig i FF.
+            unfold PrimTypeInference.find_field in FF. unfold opt_result in FF.
+            destr_in FF; inv FF.
+            revert i Heqo. simpl. destruct sig. simpl. clear.
+            induction struct_fields; intros; eauto. easy.
+            simpl. destruct a. simpl in *.
+            destr_in Heqo.
+            * inv Heqo. f_equal.
+            * destr_in Heqo; inv Heqo.
+              erewrite IHstruct_fields; eauto.
+              f_equal.
+          }
+          erewrite H; eauto. simpl. destr. destr. simpl. f_equal.
+          unfold take_drop' in Heqp.
+          edestruct (@take_drop_succeeds) as (la & lb & EQ).
+          2: rewrite EQ in Heqp.
+          rewrite vect_to_list_length.
+
+          Lemma struct_fields_sz_skipn:
+            forall n f,
+              struct_fields_sz (skipn n f) <= struct_fields_sz f.
+          Proof.
+            induction n; simpl; intros; eauto. destr. auto.
+            etransitivity. apply IHn. unfold struct_fields_sz. simpl. lia.
+          Qed.
+          Lemma field_offset_right_le:
+            forall sig s,
+              field_offset_right sig s <= struct_sz sig.
+          Proof.
+            unfold field_offset_right, struct_sz.
+            simpl type_sz.
+
+            intros; apply struct_fields_sz_skipn.
+
+          Qed.
+          apply field_offset_right_le.
+          f_equal.
+          rewrite app_length. rewrite repeat_length.
+          cut (List.length l1 <= field_sz sig s). lia.
+          apply take_drop'_spec in Heqp0. intuition.
+
+          unfold Bits.slice. rewrite vect_extend_end_firstn.
+          unfold Bits.extend_end.
+          rewrite vect_to_list_eq_rect.
+          rewrite vect_to_list_app.
+          rewrite vect_firstn_to_list.
+          rewrite vect_skipn_to_list.
+          rewrite <- repeat_bits_const.
+          unfold take_drop' at 2. rewrite EQ. simpl.
+          inv Heqp. rewrite Heqp0. simpl. f_equal. f_equal.
+          eapply take_drop'_spec2 in Heqp0. destruct Heqp0.
+          rewrite H1.
+          clear H0 H1.
+          eapply take_drop_spec in EQ. intuition.
+          rewrite H3. rewrite vect_to_list_length. reflexivity.
+      - destr_in H.
+        + repeat destr_in H; inv H. simpl in *.
+          rewrite <- vect_nth_map. rewrite <- vect_to_list_map.
+          rewrite <- vect_to_list_nth. f_equal.
+          unfold PrimTypeInference.check_index in Heqr1.
+          unfold opt_result in Heqr1. destr_in Heqr1; inv Heqr1.
+          symmetry; apply index_to_nat_of_nat. auto.
+        + destr_in H; inv H. simpl in *. destr. destr. simpl.
+          unfold PrimTypeInference.check_index in Heqr0.
+          unfold opt_result in Heqr0. destr_in Heqr0; inv Heqr0.
+          apply index_to_nat_of_nat in Heqo. subst.
+          unfold take_drop' in *.
+          edestruct @take_drop_succeeds as (la & lb & EQ). 2: rewrite EQ in Heqp.
+          rewrite vect_to_list_length. unfold array_sz. simpl. rewrite Bits.rmul_correct.
+          rewrite Nat.mul_comm. unfold element_sz. apply Nat.mul_le_mono_r.
+          cut (index_to_nat s < array_len sig). lia. eapply lt_le_trans.
+          apply index_to_nat_bounded. lia.
+          inv Heqp.
+          generalize EQ; intro EQs.
+          apply take_drop_spec in EQ. intuition.
+          edestruct @take_drop_succeeds as (la & lb & EQ'). 2: rewrite EQ' in Heqp0.
+          rewrite H2, vect_to_list_length. unfold array_sz. simpl. rewrite Bits.rmul_correct.
+          unfold element_sz.
+          (* rewrite Nat.mul_comm. unfold element_sz. apply Nat.mul_le_mono_r. *)
+          cut (index_to_nat s < array_len sig). nia.
+          apply index_to_nat_bounded.
+          f_equal. f_equal.
+          rewrite app_length, repeat_length. 
+          inv Heqp0.
+          apply take_drop_spec in EQ'. intuition.
+          inv Heqp0.
+          unfold Bits.slice. rewrite vect_extend_end_firstn.
+          unfold Bits.extend_end.
+          rewrite vect_to_list_eq_rect.
+          rewrite vect_to_list_app.
+          rewrite vect_firstn_to_list.
+          rewrite vect_skipn_to_list.
+          rewrite <- repeat_bits_const.
+          unfold take_drop' at 2.
+          unfold element_offset_right. rewrite Bits.rmul_correct.
+          rewrite Nat.mul_comm. rewrite EQs. simpl.
+          unfold take_drop'; rewrite EQ'; simpl. f_equal. f_equal.
+          eapply take_drop_spec in EQ'. intuition. rewrite H4.
+          rewrite Nat.min_l. auto.
+          unfold element_sz. unfold array_sz. simpl.
+          rewrite Bits.rmul_correct. rewrite Nat.mul_comm.
+          rewrite <- Nat.mul_sub_distr_l.
+          cut (1 <= array_len sig - (array_len sig - S (index_to_nat s))). nia.
+          generalize (index_to_nat_bounded s). lia.
+    Qed.
+
+    Definition enum_sig_eq_dec (s1 s2: enum_sig) : {s1 = s2} + {s1 <> s2}.
+    Proof.
+      destruct s1, s2; simpl.
+      destruct (eq_dec enum_name enum_name0). 2: right; intro A; inv A; congruence.
+      destruct (eq_dec enum_size enum_size0). 2: right; intro A; inv A; congruence.
+      destruct (eq_dec enum_bitsize enum_bitsize0). 2: right; intro A; inv A; congruence.
+      subst.
+      destruct (eq_dec enum_members enum_members0).
+      destruct (eq_dec enum_bitpatterns enum_bitpatterns0).
+      left; subst; reflexivity. right; intro A; inv A.
+      apply Eqdep_dec.inj_pair2_eq_dec in H1. 2: apply eq_dec.
+      apply Eqdep_dec.inj_pair2_eq_dec in H1. 2: apply eq_dec.
+      congruence.
+      right; intro A; inv A.
+      apply Eqdep_dec.inj_pair2_eq_dec in H0. 2: apply eq_dec. congruence.
+    Defined.
+
+
+    Definition struct_sig_eq_dec (s1 s2: struct_sig) : {s1 = s2} + {s1 <> s2}.
+    Proof.
+      destruct s1, s2; simpl.
+      destruct (eq_dec struct_name struct_name0). 2: right; intro A; inv A; congruence.
+      destruct (eq_dec struct_fields struct_fields0). 2: right; intro A; inv A; congruence.
+      left; subst; reflexivity.
+    Defined.
+
+    Lemma val_ind':
+      forall (P : val -> Type)
+       (Hbits: forall (n : nat) (bs : list bool), P (Bits n bs))
+       (Henum: forall (sig : enum_sig) (bs : list bool),
+           P (Enum sig bs))
+       (Hstruct: forall (sig : struct_sig) (lv : list val),
+           (forall x, In x lv -> P x) ->
+        P (Struct sig lv))
+       (Harray: forall (sig : array_sig) (lv : list val),
+           (forall x, In x lv -> P x) ->
+        P (Array sig lv)),
+      forall (v : val), P v.
+    Proof.
+      intros P Hbits Henum Hstruct Harray v.
+      remember (size_val v).
+      revert v Heqn.
+      pattern n.
+
+      Lemma strong_ind_type:
+        forall (P: nat -> Type)
+               (IH: forall n, (forall m, m < n -> P m) -> P n),
+        forall n, forall m, m <= n -> P m.
+      Proof.
+        induction n. intros. apply IH. lia.
+        intros.
+        destruct (le_dec m n); eauto.
+        assert (m = S n) by lia. clear H n0. subst.
+        apply IH. intros. apply IHn; auto. lia.
+      Qed.
+
+      eapply strong_ind_type. 2: reflexivity.
+      intros n0 Plt v Heqn.
+      assert (Plt':
+                forall v,
+                  size_val v < n0 -> P v
+             ).
+      {
+        intros. eapply Plt. 2: reflexivity. lia.
+      } clear Plt.
+      rename Plt' into Plt.
+      subst.
+      destruct v; eauto.
+      - eapply Hstruct.
+        intros.
+        eapply Plt. simpl.
+        clear Plt. revert x v H.
+        induction v; simpl; intros; eauto. easy.
+        destruct H; subst; eauto. lia.
+        eapply lt_le_trans. apply IHv; auto. lia.
+      - eapply Harray.
+        intros.
+        eapply Plt. simpl.
+        clear Plt. revert x v H.
+        induction v; simpl; intros; eauto. easy.
+        destruct H; subst; eauto. lia.
+        eapply lt_le_trans. apply IHv; auto. lia.
+    Qed.
+
+    Definition list_eq_dec' {A: Type} (l1 l2: list A) (Aeq: forall x y, In x l1 -> {x = y} + {x <> y}): {l1 = l2} + {l1 <> l2}.
+    Proof.
+      revert l1 Aeq l2; induction l1; simpl; intros.
+      - destruct l2. left; reflexivity. right; intro B; inv B.
+      - destruct l2. right; congruence.
+        destruct (Aeq a a0). simpl; auto. subst.
+        2: right; intro B; inv B; congruence.
+        edestruct (fun pf => IHl1 pf l2). intros; eauto.
+        subst. left; reflexivity.
+        right; intro B; inv B; congruence.
+    Defined.
+
+    Definition val_eq_dec (v1 v2: val) : {v1 = v2} + {v1 <> v2}.
+    Proof.
+      revert v2.
+      pattern v1. revert v1.
+      eapply val_ind'; simpl; intros.
+      - destruct v2; try (right; intro A; inv A; congruence).
+        destruct (eq_dec n sz); try (right; intro A; inv A; congruence).
+        destruct (eq_dec bs v); try (right; intro A; inv A; congruence).
+        subst; left; reflexivity.
+      - destruct v2; try (right; intro A; inv A; congruence).
+        destruct (enum_sig_eq_dec sig sig0); try (right; intro A; inv A; congruence).
+        destruct (eq_dec bs v); try (right; intro A; inv A; congruence).
+        subst; left; reflexivity.
+      - destruct v2; try (right; intro A; inv A; congruence).
+        destruct (struct_sig_eq_dec sig sig0); try (right; intro A; inv A; congruence).
+        destruct (list_eq_dec' lv v); try (right; intro A; inv A; congruence). eauto.
+        left; subst. reflexivity.
+      - destruct v2; try (right; intro A; inv A; congruence).
+        destruct (eq_dec sig sig0); subst. 2: (right; intro A; inv A; congruence).
+        destruct (list_eq_dec' lv v); try (right; intro A; inv A; congruence). eauto.
+        left; subst. reflexivity.
+    Defined.
+
+    (* Definition ubits2_sigma (ub: ubits2) (v1 v2: list bool) : list bool := *)
+    (*   match ubits2 with *)
+    (*   | UAnd =>  *)
+
+  Definition sigma2 (fn: ufn2) (v1 v2: val) : option val :=
     match fn with
-    | PrimUntyped.UDisplay fn =>
-      match fn with
-      | PrimUntyped.UDisplayUtf8 => fun _ => Some (Bits _ Ob)
-      | PrimUntyped.UDisplayValue _ => fun _ => Some (Bits _ Ob)
-      end
-    | PrimUntyped.UConv fn =>
-      match fn with
-      | PrimUntyped.UPack => fun v => Some (ubits_of_value v)
-      | PrimUntyped.UUnpack tau => fun bs => value_of_bits (tau:=tau) bs
-      | PrimUntyped.UIgnore => fun _ => Some (Bits _ Ob)
-      end
-    | PrimUntyped.UBits1 fn => CircuitPrimSpecs.sigma1 fn
-    | PrimUntyped.UStruct1 (PrimUntyped.UGetField f) =>
-      BitFuns.get_field
-
-    | PrimUntyped.UArray1 (PrimUntyped.UGetElement idx) => fun a => vect_nth a idx
+    | UEq false  => if val_eq_dec v1 v2 then Bits 1 [true] else Bits 1 [false]
+    | UEq true  => if val_eq_dec v1 v2 then Bits 1 [false] else Bits 1 [true]
+    | UBits2 fn => 
+    | Struct2 SubstField sig idx => fun s v => subst_field sig.(struct_fields) s idx v
+    | Array2 SubstElement sig idx => fun a e => vect_replace a idx e
     end.
-
-  (* Definition sigma2 (fn: fn2) : Sig_denote (PrimSignatures.Sigma2 fn) := *)
-  (*   match fn with *)
-  (*   | Eq tau false  => _eq *)
-  (*   | Eq tau true  => _neq *)
-  (*   | Bits2 fn => CircuitPrimSpecs.sigma2 fn *)
-  (*   | Struct2 SubstField sig idx => fun s v => subst_field sig.(struct_fields) s idx v *)
-  (*   | Array2 SubstElement sig idx => fun a e => vect_replace a idx e *)
-  (*   end. *)
 
 
     Fixpoint interp_action
